feat: add typeclasses for easier use of State.Typed (#19)
* feat: add typeclasses for easier use of State.Typed

* cleanup: improve type and function names in DY.Lib.State.Tagged

* cleanup: improve `map_types` instance names

* cleanup: use a dedicated type for PrivateKey's map keys

src/lib/state/DY.Lib.State.Tagged.fst
@@ -8,22 +8,22 @@ open DY.Lib.Comparse.Parsers
 
 #set-options "--fuel 1 --ifuel 1"
 
-(*** Session predicates ***)
+(*** Tagged state predicates ***)
 
 [@@ with_bytes bytes]
-type session = {
+type tagged_state = {
   [@@@ with_parser #bytes ps_string]
   tag: string;
   content: bytes;
 }
 
-%splice [ps_session] (gen_parser (`session))
-%splice [ps_session_is_well_formed] (gen_is_well_formed_lemma (`session))
+%splice [ps_tagged_state] (gen_parser (`tagged_state))
+%splice [ps_tagged_state_is_well_formed] (gen_is_well_formed_lemma (`tagged_state))
 
-instance parseable_serializeable_session: parseable_serializeable bytes session = mk_parseable_serializeable (ps_session)
+instance parseable_serializeable_tagged_state: parseable_serializeable bytes tagged_state = mk_parseable_serializeable (ps_tagged_state)
 
 noeq
-type session_pred {|crypto_invariants|} = {
+type local_bytes_state_predicate {|crypto_invariants|} = {
   pred: trace -> principal -> nat -> bytes -> prop;
   pred_later:
     tr1:trace -> tr2:trace ->
@@ -40,14 +40,14 @@ type session_pred {|crypto_invariants|} = {
   ;
 }
 
-let split_session_pred_func {|crypto_invariants|} : split_predicate_input_values = {
+let split_local_bytes_state_predicate_func {|crypto_invariants|} : split_predicate_input_values = {
   tagged_data_t = trace & principal & nat & bytes;
   tag_t = string;
   encoded_tag_t = string;
   raw_data_t = trace & principal & nat & bytes;
 
   decode_tagged_data = (fun (tr, prin, sess_id, sess_content) -> (
-    match parse session sess_content with
+    match parse tagged_state sess_content with
     | Some ({tag; content}) -> Some (tag, (tr, prin, sess_id, content))
     | None -> None
   ));
@@ -55,7 +55,7 @@ let split_session_pred_func {|crypto_invariants|} : split_predicate_input_values
   encode_tag = (fun s -> s);
   encode_tag_inj = (fun l1 l2 -> ());
 
-  local_pred = session_pred;
+  local_pred = local_bytes_state_predicate;
   global_pred = trace -> principal -> nat -> bytes -> prop;
 
   apply_local_pred = (fun spred (tr, prin, sess_id, content) ->
@@ -70,71 +70,71 @@ let split_session_pred_func {|crypto_invariants|} : split_predicate_input_values
   apply_mk_global_pred = (fun spred x -> ());
 }
 
-val has_session_pred: protocol_invariants -> (string & session_pred) -> prop
-let has_session_pred invs (tag, spred) =
-  has_local_pred split_session_pred_func (state_pred) (tag, spred)
+val has_local_bytes_state_predicate: protocol_invariants -> (string & local_bytes_state_predicate) -> prop
+let has_local_bytes_state_predicate invs (tag, spred) =
+  has_local_pred split_local_bytes_state_predicate_func (state_pred) (tag, spred)
 
-(*** Global session predicate builder ***)
+(*** Global tagged state predicate builder ***)
 
-val mk_global_session_pred: {|crypto_invariants|} -> list (string & session_pred) -> trace -> principal -> nat -> bytes -> prop
-let mk_global_session_pred #cinvs l =
-  mk_global_pred split_session_pred_func l
+val mk_global_local_bytes_state_predicate: {|crypto_invariants|} -> list (string & local_bytes_state_predicate) -> trace -> principal -> nat -> bytes -> prop
+let mk_global_local_bytes_state_predicate #cinvs l =
+  mk_global_pred split_local_bytes_state_predicate_func l
 
-val mk_global_session_pred_correct: invs:protocol_invariants -> lpreds:list (string & session_pred) -> Lemma
+val mk_global_local_bytes_state_predicate_correct: invs:protocol_invariants -> lpreds:list (string & local_bytes_state_predicate) -> Lemma
   (requires
-    invs.trace_invs.state_pred.pred == mk_global_session_pred lpreds /\
+    invs.trace_invs.state_pred.pred == mk_global_local_bytes_state_predicate lpreds /\
     List.Tot.no_repeats_p (List.Tot.map fst lpreds)
   )
-  (ensures for_allP (has_session_pred invs) lpreds)
-let mk_global_session_pred_correct invs lpreds =
-  for_allP_eq (has_session_pred invs) lpreds;
-  FStar.Classical.forall_intro_2 (FStar.Classical.move_requires_2 (mk_global_pred_correct split_session_pred_func lpreds))
+  (ensures for_allP (has_local_bytes_state_predicate invs) lpreds)
+let mk_global_local_bytes_state_predicate_correct invs lpreds =
+  for_allP_eq (has_local_bytes_state_predicate invs) lpreds;
+  FStar.Classical.forall_intro_2 (FStar.Classical.move_requires_2 (mk_global_pred_correct split_local_bytes_state_predicate_func lpreds))
 
-val mk_global_session_pred_later:
-  cinvs:crypto_invariants -> lpreds:list (string & session_pred) ->
+val mk_global_local_bytes_state_predicate_later:
+  cinvs:crypto_invariants -> lpreds:list (string & local_bytes_state_predicate) ->
   tr1:trace -> tr2:trace -> prin:principal -> sess_id:nat -> full_content:bytes -> Lemma
-  (requires mk_global_session_pred lpreds tr1 prin sess_id full_content /\ tr1 <$ tr2)
-  (ensures mk_global_session_pred lpreds tr2 prin sess_id full_content)
-let mk_global_session_pred_later cinvs lpreds tr1 tr2 prin sess_id full_content =
-  mk_global_pred_eq split_session_pred_func lpreds (tr1, prin, sess_id, full_content);
+  (requires mk_global_local_bytes_state_predicate lpreds tr1 prin sess_id full_content /\ tr1 <$ tr2)
+  (ensures mk_global_local_bytes_state_predicate lpreds tr2 prin sess_id full_content)
+let mk_global_local_bytes_state_predicate_later cinvs lpreds tr1 tr2 prin sess_id full_content =
+  mk_global_pred_eq split_local_bytes_state_predicate_func lpreds (tr1, prin, sess_id, full_content);
   eliminate exists tag lpred raw_data.
     List.Tot.memP (tag, lpred) lpreds /\
-    split_session_pred_func.apply_local_pred lpred raw_data /\
-    split_session_pred_func.decode_tagged_data (tr1, prin, sess_id, full_content) == Some (split_session_pred_func.encode_tag tag, raw_data)
-  returns mk_global_session_pred lpreds tr2 prin sess_id full_content
+    split_local_bytes_state_predicate_func.apply_local_pred lpred raw_data /\
+    split_local_bytes_state_predicate_func.decode_tagged_data (tr1, prin, sess_id, full_content) == Some (split_local_bytes_state_predicate_func.encode_tag tag, raw_data)
+  returns mk_global_local_bytes_state_predicate lpreds tr2 prin sess_id full_content
   with _. (
-    let Some (_, (_, _, _, content)) = split_session_pred_func.decode_tagged_data (tr1, prin, sess_id, full_content) in
+    let Some (_, (_, _, _, content)) = split_local_bytes_state_predicate_func.decode_tagged_data (tr1, prin, sess_id, full_content) in
     lpred.pred_later tr1 tr2 prin sess_id content;
-    mk_global_pred_eq split_session_pred_func lpreds (tr2, prin, sess_id, full_content);
-    assert(split_session_pred_func.apply_local_pred lpred (tr2, prin, sess_id, content))
+    mk_global_pred_eq split_local_bytes_state_predicate_func lpreds (tr2, prin, sess_id, full_content);
+    assert(split_local_bytes_state_predicate_func.apply_local_pred lpred (tr2, prin, sess_id, content))
   )
 
-val mk_global_session_pred_knowable:
-  cinvs:crypto_invariants -> lpreds:list (string & session_pred) ->
+val mk_global_local_bytes_state_predicate_knowable:
+  cinvs:crypto_invariants -> lpreds:list (string & local_bytes_state_predicate) ->
   tr:trace -> prin:principal -> sess_id:nat -> full_content:bytes ->
   Lemma
-  (requires mk_global_session_pred lpreds tr prin sess_id full_content)
+  (requires mk_global_local_bytes_state_predicate lpreds tr prin sess_id full_content)
   (ensures is_knowable_by (principal_state_label prin sess_id) tr full_content)
-let mk_global_session_pred_knowable cinvs lpreds tr prin sess_id full_content =
-  mk_global_pred_eq split_session_pred_func lpreds (tr, prin, sess_id, full_content);
+let mk_global_local_bytes_state_predicate_knowable cinvs lpreds tr prin sess_id full_content =
+  mk_global_pred_eq split_local_bytes_state_predicate_func lpreds (tr, prin, sess_id, full_content);
   eliminate exists tag lpred raw_data.
     List.Tot.memP (tag, lpred) lpreds /\
-    split_session_pred_func.apply_local_pred lpred raw_data /\
-    split_session_pred_func.decode_tagged_data (tr, prin, sess_id, full_content) == Some (split_session_pred_func.encode_tag tag, raw_data)
+    split_local_bytes_state_predicate_func.apply_local_pred lpred raw_data /\
+    split_local_bytes_state_predicate_func.decode_tagged_data (tr, prin, sess_id, full_content) == Some (split_local_bytes_state_predicate_func.encode_tag tag, raw_data)
   returns is_knowable_by (principal_state_label prin sess_id) tr full_content
   with _. (
-    let Some (tag, (_, _, _, content)) = split_session_pred_func.decode_tagged_data (tr, prin, sess_id, full_content) in
+    let Some (tag, (_, _, _, content)) = split_local_bytes_state_predicate_func.decode_tagged_data (tr, prin, sess_id, full_content) in
     lpred.pred_knowable tr prin sess_id content;
-    serialize_parse_inv_lemma session full_content;
-    serialize_wf_lemma session (is_knowable_by (principal_state_label prin sess_id) tr) ({tag; content})
+    serialize_parse_inv_lemma tagged_state full_content;
+    serialize_wf_lemma tagged_state (is_knowable_by (principal_state_label prin sess_id) tr) ({tag; content})
   )
 
-val mk_state_predicate: cinvs:crypto_invariants -> list (string & session_pred) -> state_predicate cinvs
+val mk_state_predicate: cinvs:crypto_invariants -> list (string & local_bytes_state_predicate) -> state_predicate cinvs
 let mk_state_predicate cinvs lpreds =
   {
-    pred = mk_global_session_pred lpreds;
-    pred_later = mk_global_session_pred_later cinvs lpreds;
-    pred_knowable = mk_global_session_pred_knowable cinvs lpreds;
+    pred = mk_global_local_bytes_state_predicate lpreds;
+    pred_later = mk_global_local_bytes_state_predicate_later cinvs lpreds;
+    pred_knowable = mk_global_local_bytes_state_predicate_knowable cinvs lpreds;
   }
 
 (*** Predicates on trace ***)
@@ -143,7 +143,7 @@ let mk_state_predicate cinvs lpreds =
 val tagged_state_was_set: trace -> string -> principal -> nat -> bytes -> prop
 let tagged_state_was_set tr tag prin sess_id content =
   let full_content = {tag; content;} in
-  let full_content_bytes = serialize session full_content in
+  let full_content_bytes = serialize tagged_state full_content in
   state_was_set tr prin sess_id full_content_bytes
 
 (*** API for tagged sessions ***)
@@ -152,14 +152,14 @@ let tagged_state_was_set tr tag prin sess_id content =
 val set_tagged_state: string -> principal -> nat -> bytes -> crypto unit
 let set_tagged_state tag prin sess_id content =
   let full_content = {tag; content;} in
-  let full_content_bytes = serialize session full_content in
+  let full_content_bytes = serialize tagged_state full_content in
   set_state prin sess_id full_content_bytes
 
 [@@ "opaque_to_smt"]
 val get_tagged_state: string -> principal -> nat -> crypto (option bytes)
 let get_tagged_state the_tag prin sess_id =
   let*? full_content_bytes = get_state prin sess_id in
-  match parse session full_content_bytes with
+  match parse tagged_state full_content_bytes with
     | None -> return None
     | Some ({tag; content;}) ->
       if tag = the_tag then return (Some content)
@@ -167,13 +167,13 @@ let get_tagged_state the_tag prin sess_id =
 
 val set_tagged_state_invariant:
   invs:protocol_invariants ->
-  tag:string -> spred:session_pred ->
+  tag:string -> spred:local_bytes_state_predicate ->
   prin:principal -> sess_id:nat -> content:bytes -> tr:trace ->
   Lemma
   (requires
     spred.pred tr prin sess_id content /\
     trace_invariant tr /\
-    has_session_pred invs (tag, spred)
+    has_local_bytes_state_predicate invs (tag, spred)
   )
   (ensures (
     let ((), tr_out) = set_tagged_state tag prin sess_id content tr in
@@ -182,22 +182,22 @@ val set_tagged_state_invariant:
   ))
   [SMTPat (set_tagged_state tag prin sess_id content tr);
    SMTPat (trace_invariant tr);
-   SMTPat (has_session_pred invs (tag, spred))]
+   SMTPat (has_local_bytes_state_predicate invs (tag, spred))]
 let set_tagged_state_invariant invs tag spred prin sess_id content tr =
   reveal_opaque (`%set_tagged_state) (set_tagged_state);
   reveal_opaque (`%tagged_state_was_set) (tagged_state_was_set);
   let full_content = {tag; content;} in
-  parse_serialize_inv_lemma #bytes session full_content;
-  local_eq_global_lemma split_session_pred_func state_pred tag spred (tr, prin, sess_id, serialize _ full_content) (tr, prin, sess_id, content)
+  parse_serialize_inv_lemma #bytes tagged_state full_content;
+  local_eq_global_lemma split_local_bytes_state_predicate_func state_pred tag spred (tr, prin, sess_id, serialize _ full_content) (tr, prin, sess_id, content)
 
 val get_tagged_state_invariant:
   invs:protocol_invariants ->
-  tag:string -> spred:session_pred ->
+  tag:string -> spred:local_bytes_state_predicate ->
   prin:principal -> sess_id:nat -> tr:trace ->
   Lemma
   (requires
     trace_invariant tr /\
-    has_session_pred invs (tag, spred)
+    has_local_bytes_state_predicate invs (tag, spred)
   )
   (ensures (
     let (opt_content, tr_out) = get_tagged_state tag prin sess_id tr in
@@ -211,7 +211,7 @@ val get_tagged_state_invariant:
   ))
   [SMTPat (get_tagged_state tag prin sess_id tr);
    SMTPat (trace_invariant tr);
-   SMTPat (has_session_pred invs (tag, spred))]
+   SMTPat (has_local_bytes_state_predicate invs (tag, spred))]
 let get_tagged_state_invariant invs tag spred prin sess_id tr =
   reveal_opaque (`%get_tagged_state) (get_tagged_state);
   let (opt_content, tr_out) = get_tagged_state tag prin sess_id tr in
@@ -219,28 +219,28 @@ let get_tagged_state_invariant invs tag spred prin sess_id tr =
   | None -> ()
   | Some content ->
     let (Some full_content_bytes, tr) = get_state prin sess_id tr in
-    local_eq_global_lemma split_session_pred_func state_pred tag spred (tr, prin, sess_id, full_content_bytes) (tr, prin, sess_id, content)
+    local_eq_global_lemma split_local_bytes_state_predicate_func state_pred tag spred (tr, prin, sess_id, full_content_bytes) (tr, prin, sess_id, content)
 
 (*** Theorem ***)
 
 val tagged_state_was_set_implies_pred:
   invs:protocol_invariants -> tr:trace ->
-  tag:string -> spred:session_pred ->
+  tag:string -> spred:local_bytes_state_predicate ->
   prin:principal -> sess_id:nat -> content:bytes ->
   Lemma
   (requires
     tagged_state_was_set tr tag prin sess_id content /\
     trace_invariant tr /\
-    has_session_pred invs (tag, spred)
+    has_local_bytes_state_predicate invs (tag, spred)
   )
   (ensures spred.pred tr prin sess_id content)
   [SMTPat (tagged_state_was_set tr tag prin sess_id content);
    SMTPat (trace_invariant tr);
-   SMTPat (has_session_pred invs (tag, spred));
+   SMTPat (has_local_bytes_state_predicate invs (tag, spred));
   ]
 let tagged_state_was_set_implies_pred invs tr tag spred prin sess_id content =
   reveal_opaque (`%tagged_state_was_set) (tagged_state_was_set);
   let full_content = {tag; content;} in
-  parse_serialize_inv_lemma #bytes session full_content;
-  let full_content_bytes: bytes = serialize session full_content in
-  local_eq_global_lemma split_session_pred_func state_pred tag spred (tr, prin, sess_id, full_content_bytes) (tr, prin, sess_id, content)
+  parse_serialize_inv_lemma #bytes tagged_state full_content;
+  let full_content_bytes: bytes = serialize tagged_state full_content in
+  local_eq_global_lemma split_local_bytes_state_predicate_func state_pred tag spred (tr, prin, sess_id, full_content_bytes) (tr, prin, sess_id, content)
